\begin{figure}
\begin{minipage}{1.0\textwidth}
\scriptsize
\begin{gather*}\label{eA1}
 \texttt{F-Form1} \frac
 { t = \textnormal{con}(t_1, \cdots,t_n) \ t \in \mathcal{T}(S) \setminus ( \mathcal{D}(F) \cup C)  \ \  N[t_1] = s_1 \cdots N[t_n] = s_n }
 { F := F, t \mapsto ( s_1, \cdots, s_n) \downarrow}\\
 \texttt{F-Form2} \frac
 { l \in \mathcal{T}(S) \setminus \mathcal{D}(F)}
 { F := F, t \mapsto ( l)} \\
  \texttt{N-Form1} \frac
  { [x] \not\in \mathcal{D}(N) \ \ s \in [x] \setminus ( C \cup \mathcal{V}(S)) \ \ F t= F s \textnormal{for all} \ t \in [x] \setminus ( C \cup \mathcal{V}(S)) }
  { N:= N, [x] \mapsto F s}\\
  \texttt{N-Form2} \frac
  { [x] \not\in \mathcal{D}(N) \ \ [x] \subseteq  C \cup \mathcal{V}(S)} 
  { N:= N, [x] \mapsto (x)}
\end{gather*}
\end{minipage}
\caption{The rules for normalization\cite{main-paper}.}
\label{rules_3}
\end{figure}