\begin{figure}
\begin{align*}
\texttt{con}(\mathbf{s},  \texttt{con}(\mathbf{t}), \mathbf{u}) &\rightarrow   \texttt{con}(\mathbf{s},\mathbf{t}, \mathbf{u})\\
\texttt{con}(\mathbf{s}, \epsilon, \mathbf{u}) &\rightarrow \texttt{con}(\mathbf{s}, \mathbf{u})\\
\texttt{con}(s) &\rightarrow s\\
\texttt{con}() &\rightarrow \epsilon\\
\texttt{con}(\mathbf{s}, c_1 \cdots c_i, c_{i+1} \cdots c_n, \mathbf{u}) &\rightarrow \texttt{con}(\mathbf{s}, c_1 \cdots c_n, \mathbf{u})\\
\texttt{len}( \texttt{con}(s_1,\cdots,s_n)) &\rightarrow \texttt{len}(s_1) + \cdots + \texttt{len}(s_n)\\
\texttt{len}(c_1,\cdots,c_n) &\rightarrow n
\end{align*}
\end{figure}